Hash ElGamal (Generic): ported.

examples/hashed_elgamal_generic.ec
@@ -1,56 +1,40 @@
-require import Pred.
-require import OldDistr.
-require import Int.
-require import Real.
-require import FMap.
-require import FSet.
-require (*--*) CDH.
-require (*--*) AWord.
-require (*--*) ROM.
-require (*--*) PKE.
+require import AllCore Int Real NewFMap FSet.
+require (*--*) BitWord Distr DInterval.
+(*---*) import StdOrder.RealOrder.
+require (*--*) DiffieHellman ROM PKE_CPA.
 
 (* The type of plaintexts: bitstrings of length k *)
-type bits.
-op k: int.
-axiom k_pos: 0 < k.
+op k: { int | 0 < k } as gt0_k.
 
-op uniform: bits distr.
-axiom uniformU: isuniform uniform.
-axiom uniformX x: mu uniform ((=) x) = 1%r/(2^k)%r.
-axiom uniformL: mu uniform True = 1%r.
-
-op (^^): bits -> bits -> bits.
-
-clone import AWord as Bitstring with
-  type word <- bits,
-  op length <- k,
-  op (^) <- (^^),
-  op Dword.dword <- uniform
-proof
-  Dword.*     by smt,
-  leq0_length by smt.
+clone import BitWord as Bits with
+  op n <- k
+proof gt0_n by exact/gt0_k
+rename
+  "word" as "bits"
+  "dunifin" as "dbits".
+import DWord.
 
 (* Upper bound on the number of calls to H *)
-op qH: int.
-axiom qH_pos: 0 < qH.
+op qH: { int | 0 < qH } as gt0_qH.
 
-(* Assumption *)
-clone import CDH.Set_CDH as SCDH with
+(* Assumption: Set CDH *)
+clone import DiffieHellman.Set_CDH as SCDH with
   op n <- qH.
+import DiffieHellman G FDistr.
 
-import Group.
+type pkey = group.
+type skey = t.
+type ptxt = bits.
+type ctxt = group * bits.
 
-type pkey       = group.
-type skey       = int.
-type plaintext  = bits.
-type ciphertext = group * bits.
-
-clone import PKE as PKE_ with
+(* Goal: PK IND-CPA *)
+clone import PKE_CPA as PKE with
   type pkey <- pkey,
   type skey <- skey,
-  type plaintext <- plaintext,
-  type ciphertext <- ciphertext.
+  type ptxt <- ptxt,
+  type ctxt <- ctxt.
 
+(* Some abstract hash oracle *)
 module type Hash = {
   proc init(): unit
   proc hash(x:group): bits
@@ -61,64 +45,60 @@ module Hashed_ElGamal (H:Hash): Scheme = {
     var sk;
 
     H.init();
-    sk = $[0..q-1];
+    sk <$ dt;
     return (g ^ sk, sk);
   }
 
-  proc enc(pk:pkey, m:plaintext): ciphertext = {
+  proc enc(pk:pkey, m:ptxt): ctxt = {
     var y, h;
 
-    y = $[0..q-1];
-    h = H.hash(pk ^ y);
-    return (g ^ y, h ^^ m);
+    y <$ dt;
+    h <@ H.hash(pk ^ y);
+    return (g ^ y, h +^ m);
   }
 
-  proc dec(sk:skey, c:ciphertext): plaintext option = {
+  proc dec(sk:skey, c:ctxt): ptxt option = {
     var gy, h, hm;
 
-    (gy, hm) = c;
-    h = H.hash(gy ^ sk);
-    return Option.Some (h ^^ hm);
+    (gy, hm) <- c;
+    h        <@ H.hash(gy ^ sk);
+    return Some (h +^ hm);
   }
 }.
 
 clone import ROM.ROM_BadCall as ROC with
   type from  <- group,
   type to    <- bits,
-  op dsample <- fun (x:group), uniform,
+  op dsample <- fun (x:group), dbits,
   op qH      <- qH
 proof * by smt.
 
 (* Adversary Definitions *)
 module type Adversary (O:ARO) = {
-  proc choose(pk:pkey)    : plaintext * plaintext
-  proc guess(c:ciphertext): bool
+  proc choose(pk:pkey): ptxt * ptxt
+  proc guess(c:ctxt)  : bool
 }.
 
 (* Specializing and merging the hash function *)
 module H:Hash = {
-  proc init(): unit = { RO.init(); Log.qs = FSet.empty; }
-  proc hash(x:group): bits = { var y; y = RO.o(x); return y; }
+  proc init(): unit = { RO.init(); Log.qs <- fset0; }
+  proc hash(x:group): bits = { var y; y <@ RO.o(x); return y; }
 }.
 
 (* The initial scheme *)
 module S = Hashed_ElGamal(H).
 
-(* Correctness result *)
-hoare Correctness: Correctness(S).main: true ==> res.
-proof. by proc; inline *; auto; progress; smt. qed.
-
 (* The reduction *)
 module SCDH_from_CPA(A:Adversary,O:Oracle): Top.SCDH.Adversary = {
   module BA = A(Bound(O))
 
-  proc solve(gx:group, gy:group): group set = {
+  proc solve(gx:group, gy:group): group fset = {
     var m0, m1, h, b';
 
     H.init();
-    (m0,m1)  = BA.choose(gx);
-    h        = $uniform;
-    b'       = BA.guess(gy, h);
+    (m0,m1)  <@ BA.choose(gx);
+    h        <$ dbits;
+    b'       <@ BA.guess(gy, h);
     return Log.qs;
   }
 }.
@@ -128,8 +108,8 @@ module SCDH_from_CPA(A:Adversary,O:Oracle): Top.SCDH.Adversary = {
 section.
   declare module A: Adversary {RO, Log, OnBound.G1, OnBound.G2}.
 
-  axiom chooseL (O <: ARO {A}): islossless O.o => islossless A(O).choose.
-  axiom guessL (O <: ARO {A}) : islossless O.o => islossless A(O).guess.
+  axiom choose_ll (O <: ARO {A}): islossless O.o => islossless A(O).choose.
+  axiom guess_ll (O <: ARO {A}) : islossless O.o => islossless A(O).guess.
 
   local module BA = A(Bound(RO)).
 
@@ -141,15 +121,15 @@ section.
       var x, y, h, gx;
 
       H.init();
-      x       = $[0..q-1];
-      y       = $[0..q-1];
-      gx      = g ^ x;
-      gxy     = gx ^ y;
-      (m0,m1) = BA.choose(gx);
-      b       = ${0,1};
-      h       = H.hash(gxy);
-      c       = (g ^ y, h ^^ (b ? m1 : m0));
-      b'      = BA.guess(c);
+      x       <$ dt;
+      y       <$ dt;
+      gx      <- g ^ x;
+      gxy     <- gx ^ y;
+      (m0,m1) <@ BA.choose(gx);
+      b       <$ {0,1};
+      h       <@ H.hash(gxy);
+      c       <- (g ^ y, h +^ (b ? m1 : m0));
+      b'      <@ BA.guess(c);
       return (b' = b);
     }
   }.
@@ -177,15 +157,15 @@ section.
       var x, y, h, gx, gxy;
 
       H.init();
-      x       = $[0..q-1];
-      y       = $[0..q-1];
-      gx      = g ^ x;
-      gxy     = gx ^ y;
-      (m0,m1) = BA.choose(gx);
-      b       = ${0,1};
-      h       = $uniform;
-      c       = (g ^ y, h ^^ (b ? m1 : m0));
-      b'      = BA.guess(c);
+      x       <$ dt;
+      y       <$ dt;
+      gx      <- g ^ x;
+      gxy     <- gx ^ y;
+      (m0,m1) <@ BA.choose(gx);
+      b       <$ {0,1};
+      h       <$ dbits;
+      c       <- (g ^ y, h +^ (b ? m1 : m0));
+      b'      <@ BA.guess(c);
       return (b' = b);
     }
   }.
@@ -198,42 +178,42 @@ section.
       var x, y, h, gx;
 
       H.init();
-      x       = $[0..q-1];
-      y       = $[0..q-1];
-      gx      = g ^ x;
-      gxy     = gx ^ y;
-      (m0,m1) = BA.choose(gx);
-      b       = ${0,1};
-      h       = $uniform;
-      c       = (g ^ y, h ^^ (b ? m1 : m0));
-      b'      = BA.guess(c);
-      return mem G2.gxy Log.qs;
+      x       <$ dt;
+      y       <$ dt;
+      gx      <- g ^ x;
+      gxy     <- gx ^ y;
+      (m0,m1) <@ BA.choose(gx);
+      b       <$ {0,1};
+      h       <$ dbits;
+      c       <- (g ^ y, h +^ (b ? m1 : m0));
+      b'      <@ BA.guess(c);
+      return G2.gxy \in Log.qs;
     }
   }.
 
-  local module D(H:ARO): ROC.Dist(H) = {
+  local module (D : ROC.Dist) (H : ARO) = {
     module A = A(H)
 
-    var y:int
+    var y:t
     var b:bool
-    var m0, m1:plaintext
+    var m0, m1:ptxt
 
     proc a1(): group = {
       var x, gxy, gx;
 
-      x       = $[0..q-1];
-      y       = $[0..q-1];
-      gx      = g ^ x;
-      gxy     = gx ^ y;
-      (m0,m1) = A.choose(gx);
-      b       = ${0,1};
+      x       <$ dt;
+      y       <$ dt;
+      gx      <- g ^ x;
+      gxy     <- gx ^ y;
+      (m0,m1) <@ A.choose(gx);
+      b       <$ {0,1};
       return gxy;
     }
 
     proc a2(x:bits): bool = {
       var c, b';
 
-      c  = (g ^ y, x ^^ (b ? m1 : m0));
+      c  = (g ^ y, x +^ (b ? m1 : m0));
       b' = A.guess(c);
       return (b' = b);
     }
@@ -271,8 +251,8 @@ section.
   proof.
     rewrite (G0_D &m) (G1_D &m) (G2_D &m).
     apply (OnBound.ROM_BadCall D _ _ &m).
-      by progress; proc; auto; call (chooseL H _)=> //; auto; progress; smt.
-      by progress; proc; call (guessL H _)=> //; auto.
+      by progress; proc; auto; call (choose_ll H _)=> //; auto; progress; smt.
+      by progress; proc; call (guess_ll H _)=> //; auto.
   qed.
 
   local module G1' = {
@@ -281,15 +261,15 @@ section.
       var x, y, h, gx, gxy;
 
       H.init();
-      x       = $[0..q-1];
-      y       = $[0..q-1];
-      gx      = g ^ x;
-      gxy     = gx ^ y;
-      (m0,m1) = BA.choose(gx);
-      b       = ${0,1};
-      h       = $uniform;
-      c       = (g ^ y, h);
-      b'      = BA.guess(c);
+      x       <$ dt;
+      y       <$ dt;
+      gx      <- g ^ x;
+      gxy     <- gx ^ y;
+      (m0,m1) <@ BA.choose(gx);
+      b       <$ {0,1};
+      h       <$ dbits;
+      c       <- (g ^ y, h);
+      b'      <@ BA.guess(c);
       return (b' = b);
     }
   }.
@@ -299,9 +279,13 @@ section.
     byequiv (_: ={glob A} ==> ={res})=> //.
     proc.
     call (_: ={glob RO, glob Log}); first by sim.
-    wp; rnd (fun h, h ^^ if b then m1 else m0){1}; rnd.
+    wp; rnd (fun h, h +^ if b then m1 else m0){1}; rnd.
     call (_: ={glob RO, glob Log}); first by sim.
-    by inline H.init RO.init; auto; progress; smt.
+    inline H.init RO.init; auto=> /> x _ y _ [m0 m1] b _; progress.
+    + by algebra.
+    + exact/dbits_funi.
+    + exact/dbits_fu.
+    by algebra.
   qed.
 
   local lemma Pr_G1' &m: Pr[G1'.main() @ &m: res] = 1%r/2%r.
@@ -312,11 +296,11 @@ section.
     swap 7 3.
     rnd ((=) b').
     call (_: true);
-      first by progress; apply (guessL O).
+      first by progress; apply (guess_ll O).
       by proc; sp; if=> //; wp; call (Log_o_ll RO _).
     auto.
     call (_: true);
-      first by progress; apply (chooseL O).
+      first by progress; apply (choose_ll O).
       by proc; sp; if=> //; wp; call (Log_o_ll RO _).
     by inline H.init RO.init; auto; progress; expect 3 smt.
   qed.
@@ -329,16 +313,16 @@ section.
       var x, y, h, gx;
 
       H.init();
-      x        = $[0..q-1];
-      y        = $[0..q-1];
-      gx       = g ^ x;
-      gxy      = gx ^ y;
-      (m0,m1)  = BA.choose(gx);
-      b        = ${0,1};
-      h        = $uniform;
-      c        = (g ^ y, h);
-      b'       = BA.guess(c);
-      return mem gxy Log.qs;
+      x        <$ dt;
+      y        <$ dt;
+      gx       <- g ^ x;
+      gxy      <- gx ^ y;
+      (m0,m1)  <@ BA.choose(gx);
+      b        <$ {0,1};
+      h        <$ dbits;
+      c        <- (g ^ y, h);
+      b'       <@ BA.guess(c);
+      return gxy \in Log.qs;
     }
   }.
 
@@ -347,9 +331,13 @@ section.
     byequiv (_: ={glob A} ==> ={res})=> //.
     proc.
     call (_: ={glob RO, glob Log}); first by sim.
-    wp; rnd (fun h, h ^^ if b then m1 else m0){1}; rnd.
+    wp; rnd (fun h, h +^ if b then m1 else m0){1}; rnd.
     call (_: ={glob RO, glob Log}); first by sim.
-    by inline H.init RO.init; auto; progress; smt.
+    inline H.init RO.init; auto=> /> x _ y _ [m0 m1] b _; progress.
+    + by algebra.
+    + exact/dbits_funi.
+    + exact/dbits_fu.
+    + by algebra.
   qed.
 
   local equiv G2'_SCDH: G2'.main ~ SCDH(SCDH_from_CPA(A,RO)).main:
@@ -386,23 +374,15 @@ section.
     by apply (G0_G1_G2 &m).
   qed.
 
-  lemma mult_inv_le_r (x y z:real) :
-    0%r < x => (1%r / x) * y <= z => y <= x * z.
-  proof.
-    move=> lt0x ledivxyz.
-    cut:= mulrMle (1%r / x * y) z x _ _; [by smt | done  |].
-    by rewrite -Real.Comm.Comm -Real.Assoc.Assoc -div_def 2:mul_div // smt.
-  qed.
-
   (** Composing reduction from CPA to SCDH with reduction from SCDH to CDH *)
   lemma Security &m:
       Pr[CPA(S,A(Bound(RO))).main() @ &m: res] - 1%r / 2%r <=
       qH%r * Pr[CDH.CDH(CDH_from_SCDH(SCDH_from_CPA(A,RO))).main() @ &m: res].
   proof.
-    apply (Trans _ (Pr[SCDH(SCDH_from_CPA(A,RO)).main() @ &m: res]));
-      first smt.
-    apply mult_inv_le_r; first smt.
-    by apply (Top.SCDH.Reduction (SCDH_from_CPA(A,RO)) &m); apply qH_pos.
+    apply (ler_trans (Pr[SCDH(SCDH_from_CPA(A,RO)).main() @ &m: res])).
+    + smt(Reduction).
+    have:= Self.SCDH.Reduction (SCDH_from_CPA(A,RO)) &m gt0_qH.    
+    smt(@Real gt0_qH).
   qed.
 end section.
 
